Minor changes

Evaluator.v
@@ -1,36 +1,36 @@
-Require Export SystemFR.Trees.
-Require Export SystemFR.Syntax.
 Require Export SystemFR.TypeErasure.
 Require Export SystemFR.Freshness.
 Require Export SystemFR.Notations.
-Import Notations.UnTyped.
-Require Export SystemFR.PrimitiveSize.
+Export Notations.UnTyped.
+
 Require Export SystemFR.SmallStep.
+
 Require Import Coq.Strings.String.
 Open Scope bool_scope.
 
-
 (* Helpers *)
-Fixpoint isNat (t : tree) : bool :=
+
+Fixpoint is_nat (t : tree) : bool :=
   match t with
     | zero => true
-    | succ t1 => (isNat t1)
+    | succ t1 => (is_nat t1)
     | _ => false
 end.
-Fixpoint isValue (t: tree) : bool :=
+
+Fixpoint is_value (t: tree) : bool :=
   match t with
     | uu => true
     | ttrue => true
     | tfalse => true
-    | pp e1 e2 => andb (isValue e1) (isValue e2)
-    | tleft e1 => (isValue e1)
-    | tright e1 => (isValue e1)
+    | pp e1 e2 => andb (is_value e1) (is_value e2)
+    | tleft e1 => (is_value e1)
+    | tright e1 => (is_value e1)
     | zero => true
-    | succ e1 => (isValue e1)
+    | succ e1 => (is_value e1)
     | notype_lambda _ => true
     | _ => false end.
 
-Definition getPair t : {t': option (tree*tree) | forall t1 t2, t' = Some (t1, t2) <-> t = pp t1 t2}.
+Definition get_pair t : {t': option (tree*tree) | forall t1 t2, t' = Some (t1, t2) <-> t = pp t1 t2}.
   Proof.
     exists ( match t with
     | pp e1 e2 => Some (e1,e2)
@@ -38,7 +38,7 @@ Definition getPair t : {t': option (tree*tree) | forall t1 t2, t' = Some (t1, t2
     destruct t; steps.
   Defined.
 
-  Definition getApp t : {t': option tree | forall t1, t' = Some t1 <-> t = notype_lambda t1}.
+  Definition get_app t : {t': option tree | forall t1, t' = Some t1 <-> t = notype_lambda t1}.
   Proof.
     exists (match t with
        | notype_lambda body => Some body
@@ -46,7 +46,7 @@ Definition getPair t : {t': option (tree*tree) | forall t1 t2, t' = Some (t1, t2
     destruct t; steps.
   Defined.
 
-  Definition getLR t : {t': option tree | forall t1, t' = Some t1 <-> (t = tleft t1 \/ t = tright t1)}.
+  Definition get_LR t : {t': option tree | forall t1, t' = Some t1 <-> (t = tleft t1 \/ t = tright t1)}.
   Proof.
     exists (match t with
        | tleft t' => Some t'
@@ -63,29 +63,29 @@ Fixpoint ss_eval (t: tree) {struct t}: (option tree) :=
     | ite tfalse t1 t2 => Some t2
     | ite t t1 t2 => option_map (fun e => ite e t1 t2) (ss_eval t)
 
-    | pp e1 e2 => match (isValue e1) with
+    | pp e1 e2 => match (is_value e1) with
                    | true => option_map (pp e1) (ss_eval e2)
                    | false => option_map (fun e => pp e e2) (ss_eval e1) end
 
-    | pi1 t => match getPair t with
+    | pi1 t => match get_pair t with
               | exist _ None _  => option_map pi1 (ss_eval t)
               | exist _ (Some (e1, e2)) _ =>
-                if (isValue e1) && (isValue e2)
+                if (is_value e1) && (is_value e2)
                 then Some e1
                 else option_map pi1 (ss_eval t) end
 
-    | pi2 t => match getPair t with
+    | pi2 t => match get_pair t with
               | exist _ None _ => option_map pi2 (ss_eval t)
               | exist _ (Some (e1, e2)) _ =>
-                if (isValue e1) && (isValue e2)
+                if (is_value e1) && (is_value e2)
                 then Some e2
                 else option_map pi2 (ss_eval t) end
 
-    | app t1 t2 => match (isValue t1) with
-                    | true => match getApp t1 with
+    | app t1 t2 => match (is_value t1) with
+                    | true => match get_app t1 with
                              | exist _ None _ => option_map (app t1) (ss_eval t2)
                              | exist _ (Some ts) _ =>
-                               if (isValue t2)
+                               if (is_value t2)
                                then Some (open 0 ts t2)
                                else option_map (app t1) (ss_eval t2) end
                     | false => option_map (fun e => app e t2) (ss_eval t1) end
@@ -97,12 +97,12 @@ Fixpoint ss_eval (t: tree) {struct t}: (option tree) :=
     | tmatch t1 t0 ts => match t1 with
                        | zero => Some t0
                        | succ t2 =>
-                         if (isValue t2)
+                         if (is_value t2)
                          then Some (open 0 ts t2)
                          else option_map (fun e => tmatch e t0 ts) (ss_eval t1)
                        | _ => option_map (fun e => tmatch e t0 ts) (ss_eval t1) end
 
-    | sum_match t tl tr => if (isValue t) then match t with
+    | sum_match t tl tr => if (is_value t) then match t with
                                    | tleft v => Some (open 0 tl v)
                                    | tright v => Some (open 0 tr v)
                                    | _ => None end
@@ -111,8 +111,8 @@ Fixpoint ss_eval (t: tree) {struct t}: (option tree) :=
     | tleft t => option_map tleft (ss_eval t)
     | tright t => option_map tright (ss_eval t)
 
-    | tsize t => if (isValue t) then Some (build_nat (tsize_semantics t)) else (option_map tsize (ss_eval t))
-    | boolean_recognizer r t => if (isValue t) then match r with
+    | tsize t => if (is_value t) then Some (build_nat (tsize_semantics t)) else (option_map tsize (ss_eval t))
+    | boolean_recognizer r t => if (is_value t) then match r with
                                                    | 0 => Some (is_pair t)
                                                    | 1 => Some (is_succ t)
                                                    | 2 => Some (is_lambda t)
@@ -138,11 +138,16 @@ Definition eval (t: tree) (k: nat): (option tree) :=
 (* Tactics *)
 Ltac destruct_sig :=
 match goal with
-  | H: _ |- context[let _ := getPair ?t in _ ]  => let fresh := fresh "getPair" in destruct (getPair t) (* eqn:fresh *)
-  | H: context[getPair ?t = _ ] |- _ => let fresh := fresh "getPair" in destruct (getPair t) (* eqn:fresh *)
-  | H: context[_ = getPair ?t ] |- _ => let fresh := fresh "getPair" in destruct (getPair t) (* eqn:fresh *)
-  | H: context[getApp ?t = _ ] |- _ => let fresh := fresh "getApp" in destruct (getApp t) (* eqn:fresh *)
-  | H: context[_ = getApp ?t ] |- _ => let fresh := fresh "getApp" in destruct (getApp t) (* eqn:fresh *)
+  | H: _ |- context[let _ := get_pair ?t in _ ]  =>
+    let fresh := fresh "get_pair" in destruct (get_pair t) (* eqn:fresh *)
+  | H: context[get_pair ?t = _ ] |- _ =>
+    let fresh := fresh "get_pair" in destruct (get_pair t) (* eqn:fresh *)
+  | H: context[_ = get_pair ?t ] |- _ =>
+    let fresh := fresh "get_pair" in destruct (get_pair t) (* eqn:fresh *)
+  | H: context[get_app ?t = _ ] |- _ =>
+    let fresh := fresh "get_app" in destruct (get_app t) (* eqn:fresh *)
+  | H: context[_ = get_app ?t ] |- _ =>
+    let fresh := fresh "get_app" in destruct (get_app t) (* eqn:fresh *)
 end. (* match on type of t = sig *)
 
 Ltac destruct_ss_eval :=
@@ -151,43 +156,54 @@ Ltac destruct_ss_eval :=
 
 
 (* Results *)
-Lemma isValueCorrect : forall v, isValue v = true <-> cbv_value v.
+Lemma is_value_correct : forall v, is_value v = true <-> cbv_value v.
 Proof.
   split.
   - induction v; repeat step || bools; eauto with values.
   - induction 1; repeat step || bools.
 Defined.
-Lemma ss_eval_step : forall t t', ss_eval t = Some t' -> isValue t = true -> False.
+
+Lemma ss_eval_step : forall t t', ss_eval t = Some t' -> is_value t = true -> False.
 Proof.
   induction t; repeat step || options.
 Qed.
+
 Ltac ss_eval_step :=
   match goal with
   |H: ss_eval ?t1 = Some ?t2 |- _ => poseNew (Mark (t1, t2) "ss_eval_step_h");
                                    pose proof  (ss_eval_step _ _ H) end.
 
 
-
-Lemma ss_eval_correct2: forall t t',(pfv t term_var = nil) -> scbv_step t t' ->  ss_eval t = Some t'.
-  intros. induction H0 ; repeat light || options || invert_constructor_equalities || ss_eval_step || destruct_sig || instantiate_eq_refl || list_utils || bools || rewrite <- isValueCorrect in * ||  eauto using fv_nil_top_level_var with smallstep values || destruct_match.
+Lemma ss_eval_correct2: forall t t',
+  pfv t term_var = nil ->
+  t ~> t' ->
+  ss_eval t = Some t'.
+Proof.
+  intros. induction H0 ; repeat light || options || invert_constructor_equalities || ss_eval_step || destruct_sig || instantiate_eq_refl || list_utils || bools || rewrite <- is_value_correct in * ||  eauto using fv_nil_top_level_var with smallstep values || destruct_match.
 Qed.
 
-Lemma ss_eval_correct1: forall t t', ss_eval t = Some t' -> (pfv t term_var = nil) -> scbv_step t t'.
+Lemma ss_eval_correct1: forall t t',
+  ss_eval t = Some t' ->
+  pfv t term_var = nil ->
+  t ~> t'.
 Proof.
-  induction t; intros ; repeat light ; destruct_ss_eval ; repeat light || options || bools || list_utils || instantiate_eq_refl || invert_constructor_equalities || rewrite isValueCorrect in * || destruct_sig || congruence ||  step_inversion cbv_value || destruct_match ; eauto using ss_eval_step, fv_nil_top_level_var with smallstep values . Qed.
+  induction t; intros ; repeat light ; destruct_ss_eval ; repeat light || options || bools || list_utils || instantiate_eq_refl || invert_constructor_equalities || rewrite is_value_correct in * || destruct_sig || congruence ||  step_inversion cbv_value || destruct_match ; eauto using ss_eval_step, fv_nil_top_level_var with smallstep values.
+Qed.
 
 (* Main theorem : the evaluator corresponds to the small call-by-value steps *)
-Theorem ss_eval_correct : forall t t', (pfv t term_var = nil) -> (ss_eval t = Some t' <-> scbv_step t t').
+Theorem ss_eval_correct : forall t t',
+  pfv t term_var = nil ->
+    ss_eval t = Some t' <-> t ~> t'.
 Proof.
-  intros. split ; eauto using ss_eval_correct1, ss_eval_correct2.
+  split; eauto using ss_eval_correct1, ss_eval_correct2.
 Qed.
 
-
 (* Extraction *)
+(*
 Require Extraction.
 
 Extraction Language Ocaml.
 Set Extraction AccessOpaque.
 
-
 Extraction "evaluator.ml" eval.
+*)
