examples/natmatch.v
@@ -3,7 +3,6 @@ Require Export SystemFR.Evaluator.
 Require Extraction.
 Import Notations.UnTyped.
 
-
 Definition natmatch_example := Eval compute in
   [|
    let pred :=
@@ -16,12 +15,13 @@ Definition natmatch_example := Eval compute in
    pred 9
     |].
 
-
 Example natmatch : (eval natmatch_example 1000) =  Some [| 8 |].
 Proof.
   native_compute; reflexivity. Qed.
 
+(*
 (* Extraction *)
 Extraction Language Ocaml.
 Set Extraction AccessOpaque.
 Extraction "natmatch.ml" natmatch_example eval.
+*)
